VerusLean/Vstd/Seq/Defs.lean
@@ -1,90 +1,137 @@
 import Std.Data.HashMap
+import Batteries.Data.List
 
 namespace Vstd
 
 /--
   Verus `Vstd` sequences. They are always finite.
 -/
-class VSeqLikeF (L : Type u → Type v)
+-- TODO: check James' LeanColls!
+class VSeqLikeF (L : Type u → Type u) -- actually `Type 0 → Type 0` would be enough
   extends
     Functor L
   where
-  empty : {α : Type u} → L α
-  new : {α : Type u} → (len : Nat) → (f : Nat → α) → L α
-  length : {α : Type u} → L α → Nat
-  get? : {α : Type u} → L α → Nat → Option α
-  get : {α : Type u} → (s : L α) → (i : Nat) → (h : i < length s) → α
-  get! : {α : Type u} → L α → Nat → α
-  push : {α : Type u} → L α → α → L α
-  update : {α : Type u} → L α → Nat → α → L α
-  extract : {α : Type u} → L α → Nat → Nat → L α
-  take : {α : Type u} → L α → Nat → L α -- return the whole seq if n > length
-  drop : {α : Type u} → L α → Nat → L α -- return the empty seq if n > length
-  add : {α : Type u} → L α → L α → L α
-  last : {α : Type u} → L α → α -- if empty, return a default value, or requires `length s > 0`?
-  first : {α : Type u} → L α → α -- same
+  toList : {α : Type u} → L α → List α
+  ofList : {α : Type u} → List α → L α
+  empty : {α : Type u} → L α := ofList []
 
-  mapEntries : {α β : Type u} → (int → α → β) → L α → L β
-  isPrefixOf : {α : Type u} → L α → L α → Bool
-  isSuffixOf : {α : Type u} → L α → L α → Bool
+  new : {α : Type u} → (len : Nat) → (f : Nat → α) → L α -- similar to List.ofFn but not the same
+  length : {α : Type u} → L α → Nat := fun s => toList s |>.length
+  get? : {α : Type u} → L α → Nat → Option α := fun s i => (toList s)[i]?
+  get [Inhabited α] : (s : L α) → (i : Nat) → (h : i < length s) → α :=
+    fun s i _ => (toList s).getD i default
+  get! [Inhabited α] : L α → Nat → α :=
+    fun s i => (toList s).getD i default
+  push : {α : Type u} → L α → α → L α :=
+    fun s a => ofList ((toList s) ++ [a]) -- inefficient, Array.push is efficient
+  update : {α : Type u} → L α → Nat → α → L α :=
+    fun s i a => ofList ((toList s).set i a)
+  extract : {α : Type u} → L α → Nat → Nat → L α :=
+    fun s i j => ofList ((toList s).extract i j)
+  take : {α : Type u} → L α → Nat → L α := -- return the whole seq if n > length
+    fun s n => ofList ((toList s).take n)
+  drop : {α : Type u} → L α → Nat → L α := -- return the empty seq if n > length
+    fun s n => ofList ((toList s).drop n)
+  add : {α : Type u} → L α → L α → L α :=
+    fun s₁ s₂ => ofList ((toList s₁) ++ (toList s₂))
+  last [Inhabited α] : L α → α := -- if empty, return a default value, or requires `length s > 0`?
+    fun s => (toList s).getLastD default
+  first [Inhabited α] : L α → α := -- same
+    fun s => (toList s).headD default
+
+  mapEntries : {α β : Type u} → (Nat → α → β) → L α → L β :=
+    fun f s => ofList ((toList s).zipIdx.map fun (x,i) => f i x)
+  isPrefixOf [BEq α] : L α → L α → Bool :=
+    fun s₁ s₂ => (toList s₁).isPrefixOf (toList s₂)
+  isSuffixOf [BEq α] : L α → L α → Bool :=
+    fun s₁ s₂ => (toList s₁).isSuffixOf (toList s₂)
   sortBy : {α : Type u} → (α → α → Bool) → L α → L α
-  filter : {α : Type u} → (L α) → (α → Bool) → L α
-  maxVia : {α : Type u} → (L α) → (α → α → Bool) → α
-  minVia : {α : Type u} → (L α) → (α → α → Bool) → α
-  mem : {α : Type u} → (L α) → α → Prop
-  indexOf : {α : Type u} → (L α) → α → Int
-  indexOfFirst : {α : Type u} → (L α) → α → Option Int
-  firstIndexHelper : {α : Type u} → (L α) → α → Int
-  indexOfLast : {α : Type u} → (L α) → α → Option Int
-  lastIndexHelper : {α : Type u} → (L α) → α → Int
-  dropLast : {α : Type u} → L α → L α
-  dropFirst : {α : Type u} → L α → L α
-  noDuplicates : {α : Type u} → L α → Bool
-  disjoint : {α : Type u} → L α → L α → Bool
-  insert : {α : Type u} → L α → Int → α → L α
-  remove : {α : Type u} → L α → Int → L α
-  removeValue : {α : Type u} → L α → α → L α
-  reverse : {α : Type u} → L α → L α
-  zipWith : {α β : Type u} → L α → L β → L (α × β)
-  foldLeft : {α β : Type u} → L α → β → (β → α → β) → β
-  foldLeftAlt : {α β : Type u} → L α → β → (β → α → β) → β
-  foldRight : {α β : Type u} → L α → (α → β → β) → β → β
-  foldRightAlt : {α β : Type u} → L α → (α → β → β) → β → β
-  updateSubrangeWith : {α : Type u} → L α → Int → L α → L α
+  filter : {α : Type u} → (L α) → (α → Bool) → L α :=
+    fun s p => ofList ((toList s).filter p)
+  maxVia [Inhabited α] : (L α) → (α → α → Bool) → α
+  minVia [Inhabited α] : (L α) → (α → α → Bool) → α
+  mem : {α : Type u} → (L α) → α → Prop :=
+    fun s a => a ∈ (toList s)
+  indexOf [BEq α] : (L α) → α → Int :=
+    fun s a => (toList s).idxOf a
+  indexOfFirst [BEq α] : (L α) → α → Option Int :=
+    fun s a => (toList s).idxOf? a
+  -- firstIndexHelper : {α : Type u} → (L α) → α → Int
+  indexOfLast [BEq α] : (L α) → α → Option Int
+  -- lastIndexHelper : {α : Type u} → (L α) → α → Int
+  dropLast : {α : Type u} → L α → L α :=
+    fun s => ofList ((toList s).dropLast)
+  dropFirst : {α : Type u} → L α → L α :=
+    fun s => ofList ((toList s).tail)
+  noDuplicates : {α : Type u} → L α → Prop :=
+    fun s => (toList s).Nodup
+  disjoint : {α : Type u} → L α → L α → Prop :=
+    fun s₁ s₂ => (toList s₁).Disjoint (toList s₂)
+  insert : {α : Type u} → L α → Nat → α → L α :=
+    fun s i a => ofList ((toList s).insertIdx i a)
+  remove : {α : Type u} → L α → Nat → L α :=
+    fun s i => ofList ((toList s).eraseIdx i)
+  removeValue [BEq α] : L α → α → L α :=
+    fun s a => ofList ((toList s).erase a)
+  reverse : {α : Type u} → L α → L α :=
+    fun s => ofList ((toList s).reverse)
+  zipWith : {α β : Type u} → L α → L β → L (α × β) := -- if different lengths, returns an empty sequence
+    fun s₁ s₂ => if length s₁ ≠ length s₂ then empty else ofList ((toList s₁).zip (toList s₂))
+  foldLeft : {α β : Type u} → L α → β → (β → α → β) → β :=
+    fun s init f => (toList s).foldl f init -- not the same implementation as in Verus
+  foldLeftAlt : {α β : Type u} → L α → β → (β → α → β) → β :=
+    fun s init f => (toList s).foldl f init
+  foldRight : {α β : Type u} → L α → (α → β → β) → β → β :=
+    fun s f init => (toList s).foldr f init -- not the same implementation as in Verus
+  foldRightAlt : {α β : Type u} → L α → (α → β → β) → β → β :=
+    fun s f init => (toList s).foldr f init
+  updateSubrangeWith : {α : Type u} → L α → Nat → L α → L α :=
+    fun s i t => ofList ((toList s).take i ++ (toList t) ++ (toList s).drop (i + length t))
 
-
--- #check List.get
--- #check List.get?
--- #check List.get!
--- #check List.getD
--- #check List.IsPrefix
--- #check List.isPrefixOf
--- #check Array.isPrefixOf
-
+  unzip : {α β : Type u} → L (α × β) → L α × L β :=
+    fun s => (ofList ((toList s).unzip.fst), ofList ((toList s).unzip.snd))
+  flatten : {α : Type u} → L (L α) → L α :=
+    fun s => ofList ((toList s).map toList |>.flatten)
+  flatten_alt : {α : Type u} → L (L α) → L α :=
+    fun s => ofList ((toList s).map toList |>.flatten) -- not the same implementation as in Verus
+/-
+  max [Inhabited α] [Max α] : L α → α :=
+    fun s => (toList s).max?.get!
+  min [Inhabited α] [Min α] : L α → α :=
+    fun s => (toList s).min?.get!
+  sort : {α : Type u} → L α → L α -- there is Array.qsort but no List.qsort
+  merge_sorted_with : {α : Type u} → L α → L α → (α → α → Bool) → L α
+  -- seq_to_set_rec
+ -/
 namespace VSeqLikeF
 
-variable {L : Type u → Type v} [VSeqLikeF L]
+variable {L : Type u → Type u} [VSeqLikeF L]
 
 instance instEmptyCollection : EmptyCollection (L α) := ⟨empty⟩
 instance instInhabited : Inhabited (L α) := ⟨∅⟩
 -- instance instSingleton : Singleton α (L α) := ⟨singleton⟩
 instance instMembership : Membership α (L α) := ⟨mem⟩
 instance instHAdd : HAdd (L α) (L α) (L α) := ⟨add⟩
--- instance instCoeList : Coe (List α) (S α) := ⟨ofList⟩
-instance instGetElem : GetElem (L α) Nat α (fun s i => i < length s) := ⟨get⟩
-instance instGetElem? : GetElem? (L α) Nat α (fun s i => i < length s) where
+instance instCoeList : Coe (List α) (L α) := ⟨ofList⟩
+instance instGetElem [Inhabited α] : GetElem (L α) Nat α (fun s i => i < length s) := ⟨get⟩
+instance instGetElem? [Inhabited α] : GetElem? (L α) Nat α (fun s i => i < length s) where
   getElem? := get?
   getElem! := get!
 
 end VSeqLikeF
 
+-- 1. L α is isomorphic to List α, toList, ofList, empty = ofList [], append s t = ofList (List.append (toList s) (toList t)), or say, toList (append s t) = List.append (toList s) (toList t)
+-- 2. current approach
+-- when you want to show List is an instance of Seq
 
 open VSeqLikeF in
-class LawfulVSeqLikeF (L : Type u → Type v) [VSeqLikeF L]
+class LawfulVSeqLikeF (L : Type u → Type u) [VSeqLikeF L]
   extends
     LawfulFunctor L
   where
   protected ext (s₁ s₂ : L α) : (length s₁ = length s₂ ∧ ∀ i, i < length s₁→ get? s₁ i = get? s₂ i) → s₁ = s₂
+  bla : ∀ {α : Type u} (s : L α), ofList (toList s) = s
+  ax_empty : [] = toList (empty : L α)
 
   length_empty : length (empty : L α) = 0
   length_new {α : Type u} (len : Nat) (f : Nat → α) : length (new len f : L α) = len
@@ -99,8 +146,6 @@ class LawfulVSeqLikeF (L : Type u → Type v) [VSeqLikeF L]
   length_last {α : Type u} (s : L α) (h : length s > 0) : length (dropLast s) = length s - 1
   length_first {α : Type u} (s : L α) (h : length s > 0) : length (dropFirst s) = length s - 1
   length_map {α β} (f : α → β) (s : L α) : length (f <$> s) = length s
-  -- length_filter {α} (s : L α) (p : α → Bool) : length (filter s p) ≤ length s
-
 
   get?_empty {α} (i : Nat) : get? (empty : L α) i = none
   get?_push {α} (s : L α) (a : α) (i : Nat) :
@@ -115,9 +160,9 @@ class LawfulVSeqLikeF (L : Type u → Type v) [VSeqLikeF L]
     get? (drop s n) i = get? s (n + i)
   get?_add {α} (s₁ s₂ : L α) (i : Nat) :
     get? (s₁ + s₂) i = if i < length s₁ then get? s₁ i else get? s₂ (i - length s₁)
-  get?_last {α} (s : L α) (h : length s > 0) : get? s (length s - 1) = some (last s)
-  get?_first {α} (s : L α) (h : length s > 0) : get? s 0 = some (first s)
-  get?_map {α β} (f : α → β) (s : L α) (i : Nat) :
+  get?_last {α} [Inhabited α] (s : L α) (h : length s > 0) : get? s (length s - 1) = some (last s)
+  get?_first {α} [Inhabited α] (s : L α) (h : length s > 0) : get? s 0 = some (first s)
+  get?_map {α β} [Inhabited α] (f : α → β) (s : L α) (i : Nat) :
     get? (f <$> s) i = if i < length s then some (f (get! s i)) else none
 
   extract_eq {α} (s : L α) (i j : Nat) :
@@ -132,9 +177,9 @@ class LawfulVSeqLikeF (L : Type u → Type v) [VSeqLikeF L]
   -- filter_pred {α} (s : L α) (p : α → Bool) (h : i < length (filter s p)) :
     -- p (get (filter s p) i h)
 
-  eq_push_last {α} (s : L α) (h : length s > 0) :
+  eq_push_last {α} [Inhabited α] (s : L α) (h : length s > 0) :
     (push (dropLast s) (last s)) = s
-  eq_push_first_to_drop_first {α} (s : L α) (h : length s > 0) :
+  eq_push_first_to_drop_first {α} [Inhabited α] (s : L α) (h : length s > 0) :
     (push (dropFirst s) (first s)) = s
 
   dropLast_eq {α} (s : L α) (h : length s > 0) :
@@ -142,24 +187,9 @@ class LawfulVSeqLikeF (L : Type u → Type v) [VSeqLikeF L]
   dropFirst_eq {α} (s : L α) (h : length s > 0) :
     dropFirst s = extract s 1 (length s)
 
-  -- not_mem_empty : ∀ (a : α), a ∉ (∅ : S α)
-  -- mem_insert_iff {a b : α} {s : S α} : b ∈ (s + a) ↔ b = a ∨ b ∈ s
-  -- mem_remove_iff {a b : α} {s : S α} : b ∈ (s - a) ↔ b ≠ a ∧ b ∈ s
-  -- mem_singleton_iff {a b : α} : b ∈ ({a} : S α) ↔ b = a
-  -- -- choose_mem {α : Type u} [Inhabited α] : ∀ (s : S α) (h : ∃ x, x ∈ s), choose s h ∈ s
-  -- choose_mem {α : Type u} [Inhabited α] : ∀ (s : S α), (h : ∃ x, x ∈ s) → choose s ∈ s
-  -- subset_iff {s₁ s₂ : S α} : s₁ ⊆ s₂ ↔ ∀ a, a ∈ s₁ → a ∈ s₂
-  -- mem_union_iff  {a : α} {s₁ s₂ : S α} : a ∈ s₁ ∪ s₂ ↔ a ∈ s₁ ∨ a ∈ s₂
-  -- mem_inter_iff  {a : α} {s₁ s₂ : S α} : a ∈ s₁ ∩ s₂ ↔ a ∈ s₁ ∧ a ∈ s₂
-  -- mem_sdiff_iff  {a : α} {s₁ s₂ : S α} : a ∈ s₁ \ s₂ ↔ a ∈ s₁ ∧ a ∉ s₂
-  -- mem_symmDiff_iff {a : α} {s₁ s₂ : S α} : a ∈ symmDiff s₁ s₂ ↔ (a ∈ s₁ \ s₂ ∨ a ∈ s₂ \ s₁)
-  -- disjoint_iff {s₁ s₂ : S α} : disjoint s₁ s₂ ↔ ∀ a, a ∉ s₁ ∩ s₂
-  -- mem_filter_iff {p : α → Bool} {s : S α} {a : α} : a ∈ filter s p ↔ a ∈ s ∧ p a
-  -- mem_ofList_iff {a : α} {l : List α} : a ∈ (ofList l : S α) ↔ a ∈ l
-  -- mem_map_iff {f : α → β} {s : S α} {b : β}
-  --   : b ∈ f <$> s ↔ ∃ a, a ∈ s ∧ f a = b
-  -- mem_filterMap_iff {α β : Type u} {f : α → Option β} {s : S α} {b : β}
-  --   : b ∈ filterMap f s ↔ ∃ a, a ∈ s ∧ f a = some b
+-- TODO: write definitions outside the type class, e.g. unzip via map
+def unzip {α β : Type u} [VSeqLikeF L] (s : L (α × β)) : L α × L β :=
+  (Functor.map Prod.fst s, Functor.map Prod.snd s)
 
 open LawfulVSeqLikeF in
 -- attribute [simp] not_mem_empty mem_singleton_iff mem_ofList_iff
@@ -176,23 +206,23 @@ open Std in
 def SeqVstdTranslationNames : HashMap Lean.Name Lean.Name := HashMap.ofList <|
   List.map (f := fun ⟨x, y⟩ => (String.toName s!"Vstd.Seq.{x}", String.toName y)) <| [
   /- from seq.rs -/
-  ("empty", ""),
-  ("new", ""),
-  ("len", ""),
-  ("index", ""), -- how to support direct indexing s[i]?
-  ("spec_index", ""), -- same as index
-  ("push", ""),
-  ("update", ""),
+  ("empty", "VSeqLikeF.empty"),
+  ("new", "VSeqLikeF.new"),
+  ("len", "VSeqLikeF.length"),
+  ("index", "VSeqLikeF.get!"), -- direct indexing s[i] is supported via getElem
+  ("spec_index", "VSeqLikeF.get!"), -- same as index
+  ("push", "VSeqLikeF.push"),
+  ("update", "VSeqLikeF.update"),
   ("subrange", "VSeqLikeF.extract"),
   ("take", "VSeqLikeF.take"),
   ("skip", "VSeqLikeF.drop"),
-  ("add", ""),
-  ("spec_add", ""), -- same as add
-  ("last", ""),
-  ("first", ""),
+  ("add", "VSeqLikeF.add"),
+  ("spec_add", "VSeqLikeF.add"), -- same as add
+  ("last", "VSeqLikeF.last"),
+  ("first", "VSeqLikeF.first"),
 
   /- from seq_lib.rs -/
-  ("map", ""), -- Verus TODO: rename to `map_entries`?
+  ("map", "VSeqLikeF.mapEntries"), -- Verus TODO: rename to `map_entries`?
   ("map_values", "Functor.map"), -- Verus TODO: rename to `map`?
   ("is_prefix_of", ""),
   ("is_suffix_of", ""),
@@ -223,6 +253,15 @@ def SeqVstdTranslationNames : HashMap Lean.Name Lean.Name := HashMap.ofList <|
   ("fold_right_alt", ""),
   ("update_subrange_with", ""),
 
-  -- currently ignore the functions in `impl<A, B> Seq<(A, B)>`, `impl<A> Seq<Seq<A>>`, and `impl Seq<int>`
+  ("unzip", "VSeqLikeF.unzip"),
+  ("flatten", "VSeqLikeF.flatten"),
+  ("flatten_alt", "VSeqLikeF.flatten_alt"),
+
+  ("max", "VSeqLikeF.max"),
+  ("min", "VSeqLikeF.min"),
+  ("sort", "VSeqLikeF.sort"),
+  ("merge_sorted_with", "VSeqLikeF.merge_sorted_with"),
+
+  ("seq_to_set_rec", ""),
   ]
 end Vstd
