VerusLean/Vstd/Seq/Shim.lean
@@ -2,4 +2,35 @@ import VerusLean.Vstd.Seq.Defs
 
 namespace Vstd
 
+inductive Seq (α : Type u)
+  | mk (elems : List α)
+deriving Repr, DecidableEq, Inhabited
+
+instance L : VSeqLikeF Seq where
+  map := fun f s => match s with | .mk elems => .mk (elems.map f)
+  toList := fun s => match s with | .mk elems => elems
+  ofList := fun elems => .mk elems
+  new := fun len f =>
+    .mk (List.range len |>.map f) -- incorrect
+  sortBy := fun cmp s => s
+  maxVia := fun s cmp => default -- incorrect
+  minVia := fun s cmp => default -- incorrect
+  indexOfLast := fun s a => match s with
+    | .mk elems => elems.reverse.idxOf? a
+  -- foldLeft := S.foldLeftAlt -- slightly incorrect
+  -- foldRight := S.foldRightAlt -- slightly incorrect
+  -- flatten_alt := S.flatten -- slightly incorrect
+  /-fail to show termination for
+      Vstd.S
+    with errors
+    failed to infer structural recursion:
+    no parameters suitable for structural recursion
+
+    well-founded recursion cannot be used, 'Vstd.S' does not take any (non-fixed) arguments
+    -/
+  --  => S.ofList ((S.toList s).map S.toList |>.flatten)
+
+def sort {L : Type u → Type u} [VSeqLikeF L] (s : L α) : L α := sorry
+
+
 end Vstd
